Phi_Semantics/PhiSem_Variable.thy
@@ -321,7 +321,7 @@ subsubsection \<open>Get\<close>
 proc (nodef) op_get_var:
   assumes [unfolded \<phi>SemType_def subset_iff, useful]: \<open>\<phi>SemType (x \<Ztypecolon> T) TY\<close>
   input  \<open>x \<Ztypecolon> \<v>\<a>\<r>[var] T\<close>
-  output \<open>x \<Ztypecolon> \<v>\<a>\<r>[var] T\<heavy_comma> x \<Ztypecolon> \<v>\<a>\<l> T\<close>
+  output \<open>x \<Ztypecolon> \<v>\<a>\<r>[var] T\<heavy_comma> x \<Ztypecolon> \<v>\<a>\<l> T\<close> 
   \<medium_left_bracket> to Identity op_get_var'' \<medium_right_bracket>. .
 
 lemma [\<phi>reason 1200]:
