Phi_System/Phi_Types.thy
@@ -63,7 +63,7 @@ lemma [\<phi>reason 1200]:
 
 
 subsection \<open>Func\<close>
-
+ 
 definition \<phi>Fun :: \<open>('a \<Rightarrow> 'c) \<Rightarrow> ('c,'a) \<phi>\<close>
   where [\<phi>defs]: \<open>\<phi>Fun f x = { f x }\<close>
 
@@ -126,10 +126,10 @@ subsection \<open>Stepwise Abstraction\<close>
 
 definition \<phi>Composition :: \<open>('v,'a) \<phi> \<Rightarrow> ('a,'b) \<phi> \<Rightarrow> ('v,'b) \<phi>\<close> (infixl "\<Zcomp>" 30)
   where [\<phi>defs]: \<open>\<phi>Composition T U x = (y \<Ztypecolon> T \<s>\<u>\<b>\<j> y. y \<in> (x \<Ztypecolon> U))\<close>
-
+   
 lemma [\<phi>reason 1200]:
   \<open>x \<Ztypecolon> T \<Zcomp> U \<i>\<m>\<p>\<l>\<i>\<e>\<s> y \<Ztypecolon> T \<s>\<u>\<b>\<j> y. y \<in> (x \<Ztypecolon> U) @action to RAW\<close>
-  \<medium_left_bracket> destruct\<phi> _ \<medium_right_bracket>. .
+  \<medium_left_bracket> destruct\<phi> _ thm useful  \<medium_right_bracket>. .
 
 lemma [\<phi>reason 1200]:
   \<open> y \<Ztypecolon> Identity \<i>\<m>\<p>\<l>\<i>\<e>\<s> x \<Ztypecolon> U \<a>\<n>\<d> P
